src/mqtt-packet-parser/src/disconnect.fst
@@ -11,7 +11,7 @@ module U8 = FStar.UInt8
 module U16 = FStar.UInt16
 module U32 = FStar.UInt32
 module B = LowStar.Buffer
-#set-options "--z3rlimit 10000 --initial_fuel 10 --initial_ifuel 10"
+#set-options "--z3rlimit 1000 --max_fuel 5 --max_ifuel 5"
 
 val assemble_disconnect_struct: s: struct_disconnect_parts
   -> Stack (r: struct_fixed_header)
